\documentclass[12pt]{article}

\usepackage{epsfig}
\usepackage{amsmath,amsthm,amssymb}
\usepackage{bbm}
\usepackage{graphicx}
\usepackage{float}
\usepackage{hyperref}




\usepackage{listings}
\usepackage{amsmath} % For the array environment


% These lines describe the environments we will use: Lemma and Theorem
% Although may sound repetitive to declare that our lemma will be displayed as Lemma
% it is needed so that LaTeX can write documents in other languages 
\newtheorem{lemma}{Lemma}
\newtheorem{theorem}{Theorem}

% The commands below change the bold text where it says "Section" into "Question"
\usepackage{titlesec}
\titleformat{\section}
{\normalfont\Large\bfseries}{Question~\thesection:}{1em}{}

%Commands below change page margins (this much space at the titlepage, etc)
\newlength{\toppush}
\setlength{\toppush}{2\headheight}
\addtolength{\toppush}{\headsep}

%Name and subject of the class
\def\subjnum{Math 166}
\def\subjname{Statistics}

%Name of the student, university name and which semester
\def\doheading#1#2#3{\vfill\eject\vspace*{-\toppush}%
  \vbox{\hbox to\textwidth{{\bf} \subjnum: \subjname \hfil Cooper Golemme}%
    \hbox to\textwidth{{\bf} Tufts University, Fall 2024 \hfil#3\strut}%
    \hrule}}

%Command for the title of the document (Homework 0)
\newcommand{\htitle}[1]{\vspace*{1.25ex plus 1ex minus 0ex}%
\begin{center}
{\large\bf #1}
\end{center}} 


%%%%%%%%%%%%%%%%%%%%%%%%%%%%%%%%%%%%%%%%%%%%%%%%%%%%%%%%%%%%%%%%%%%
% BEGIN DOCUMENT
%%%%%%%%%%%%%%%%%%%%%%%%%%%%%%%%%%%%%%%%%%%%%%%%%%%%%%%%%%%%%%%%%%%
\doheading{2}{title}{Homework 8}

\begin{document}

\section{Chapter 15 \#1}
Prove:
\begin{enumerate}
    \item \( Y \perp Z \).
    \item \( \psi = 1 \).
    \item \( \gamma = 0 \).
    \item For \( i, j \in \{0, 1\} \), \( p_{ij} = p_{i\cdot} p_{\cdot j} \).
\end{enumerate}



\pagebreak
\section{Chapter 15 \#4}
The \textit{New York Times} (January 8, 2003, page A12) reported the following data on death sentencing and race, from a study in Maryland:

\begin{center}
\begin{tabular}{|c|c|c|}
\hline
 & \textbf{Death Sentence} & \textbf{No Death Sentence} \\
\hline
\textbf{Black Victim} & 14 & 641 \\
\hline
\textbf{White Victim} & 62 & 594 \\
\hline
\end{tabular}
\end{center}

Analyze the data using the tools from this chapter. Interpret the results. Explain why, based only on this information, you canâ€™t make causal conclusions. (The authors of the study did use much more information in their full report.)

\textbf{Answer:}

This problem can be represented as two binary random variables. We can say that the random variable $Y = 0$ if a death sentence is issued and $Y = 1$ if a death sentence is not issued and the random variable $Z = 0$ if the victim is black and $Z = 1$ if the victim is white.

Let $X = (X_{00}, X_{01}, X_{10}, X_{11})$ be the vector of counts as in the table below (where Y is the random variable for death sentence and Z for race)

\begin{center}
\begin{tabular}{|c|c|c|c|}
\hline
 & $Y = 0$ & $Y = 1$ & \\ 
\hline
$Z = 0$ & $X_{00}$ & $X_{01}$ & $X_{0\cdot}$ \\ 
\hline
$Z = 1$ & $X_{10}$ & $X_{11}$ & $X_{1\cdot}$ \\ 
\hline
 & $X_{\cdot 0}$ & $X_{\cdot 1}$ & $n = X_{\cdot\cdot}$ \\ 
\hline
\end{tabular}
\end{center}

We are interested in measuring the vector of counts $X$. We know that each entry in $X$ has a certain probability of occuring, which we can denote $p_{ij} = \mathbb{P}(Y = i, Z = j)$ and the vector $p = (p_{00}, p_{01}, p_{10}, p_{11})$

Thus, as $X$ is a vector of counts, distributed accordingly by the vector $p$, we can say $X \sim Multinomial(n, p)$. We can now use Pearson's $\chi^2$ test statistic for independence:
\[
    U = \sum_{i=0}^1\sum_{j=0}^1 \frac{(X_{ij} - E_{ij})^2}{E_{ij}}
\]

Where, $E_{ij} = \frac{X_{\cdot j}X_{i\cdot}}{n}$

\pagebreak

Filling in the data for the count table, we get:


\begin{center}
\begin{tabular}{|c|c|c|c|}
\hline
 & $Y = 0$ & $Y = 1$ & \\ 
\hline
$Z = 0$ & 14 & 641 & 655 \\ 
\hline
$Z = 1$ & 62 & 594 & 656 \\ 
\hline
 & 76 & 1235 & 1311 \\ 
\hline
\end{tabular}
\end{center}


% \begin{align}
%      & U = \sum_{i=0}^1\sum_{j=0}^1 \frac{(X_{ij} - 1)^2}{1}\\
%      & U = \sum_{i=0}^1\sum_{j=0}^1 (X_{ij} - 1)^2\\
%      & \sum_{i=0}^1\sum_{j=0}^1 (X_{ij} - 1)^2 = \sum_{i=0}^1 (X_{i0} - 1)^2 + (X_{i1} - 1)^2\\
%      & = (X_{00} - 1)^2 + (X_{10} - 1)^2 + (X_{01} - 1)^2 + (X_{11} - 1)^2 \\
%      & = (X_{00} - 1)^2 + (X_{10} - 1)^2 + (X_{01} - 1)^2 + (X_{11} - 1)^2 \\
% \end{align}

\end{document}
